rt spec+proof: consolidate ASpec and Haskell versions of isSchedulable
This rephrases the ASpec predicate schedulable in terms of projections,
removing the monadic function is_schedulable and the auxiliary function
is_schedulable_opt.

The Haskell function isSchedulable was replaced with a reader monad
function readSchedulable and its nondet state monad counterpart
getSchedulable. A new Refine level predicate schedulable' is stated
in terms of projections, replacing isSchedulable_bool.

The preconditions of some top-level Hoare triples were simplified.

Signed-off-by: Michael McInerney <michael.mcinerney@proofcraft.systems>

spec/haskell/src/SEL4/API/Syscall.lhs
@@ -243,6 +243,8 @@ The following function implements the "Send" and "Call" system calls. It determi
 >        "Assert that `ct_not_inQ s` holds"
 >     stateAssert valid_idle'_asrt
 >         "Assert that `valid_idle' s` holds"
+>     stateAssert cur_tcb'_asrt
+>         "Assert that `cur_tcb' s` holds"
 >     thread <- withoutPreemption getCurThread
 >     info <- withoutPreemption $ getMessageInfo thread
 >     syscall
