proof/invariant-abstract/ARM/ArchVSpaceEntries_AI.thy
@@ -1170,7 +1170,7 @@ lemma perform_page_directory_valid_pdpt[wp]:
 
 crunch invoke_sched_context
  for valid_pdpt_objs[wp]: "valid_pdpt_objs::det_state \<Rightarrow> _"
-  (wp: mapM_x_wp' hoare_drop_imps hoare_vcg_if_lift2 simp: is_schedulable_def)
+  (wp: mapM_x_wp' hoare_drop_imps hoare_vcg_if_lift2)
 
 crunch end_timeslice
  for valid_pdpt_objs[wp]: "valid_pdpt_objs::det_state \<Rightarrow> _"
@@ -1700,7 +1700,7 @@ lemma call_kernel_valid_pdpt[wp]:
          apply (rule valid_validE)
          apply (wpsimp)
          apply (fastforce simp: ct_in_state_def pred_tcb_weakenE)
-        apply (wpsimp wp: is_schedulable_wp hoare_vcg_all_lift hoare_drop_imps hoare_vcg_if_lift2)
+        apply (wpsimp wp: hoare_vcg_all_lift hoare_drop_imps hoare_vcg_if_lift2)
        apply wpsimp
     (***)
       apply (rule_tac Q'="\<lambda>_. (\<lambda>s. \<forall>x\<in>ran (kheap s). obj_valid_pdpt x)" in bind_wp_fwd)
@@ -1710,7 +1710,9 @@ lemma call_kernel_valid_pdpt[wp]:
            (\<lambda>s. \<forall>x\<in>ran (kheap s). obj_valid_pdpt x) and
            (\<lambda>s. bound_sc_tcb_at (\<lambda>a. \<exists>y. a = Some y) (cur_thread s) s)" in bind_wp_fwd)
         apply wpsimp
-        apply (clarsimp simp: pred_tcb_at_def obj_at_def schedulable_def')
+        apply (clarsimp simp: pred_tcb_at_def obj_at_def schedulable_def opt_pred_def opt_map_def
+                              tcbs_of_kh_def
+                       split: option.splits)
        apply (rule_tac Q'="\<lambda>rv. invs and (\<lambda>s. rv \<longrightarrow> ct_running s) and
            (\<lambda>s. \<forall>x\<in>ran (kheap s). obj_valid_pdpt x)" in bind_wp_fwd)
         apply (wpsimp wp: check_budget_restart_true)
@@ -1723,7 +1725,9 @@ lemma call_kernel_valid_pdpt[wp]:
            (\<lambda>s. \<forall>x\<in>ran (kheap s). obj_valid_pdpt x) and
            (\<lambda>s. bound_sc_tcb_at (\<lambda>a. \<exists>y. a = Some y) (cur_thread s) s)" in bind_wp_fwd)
        apply wpsimp
-       apply (clarsimp simp: pred_tcb_at_def obj_at_def schedulable_def')
+       apply (clarsimp simp: pred_tcb_at_def obj_at_def schedulable_def opt_pred_def opt_map_def
+                             tcbs_of_kh_def
+                      split: option.splits)
       apply (rule_tac Q'="\<lambda>rv. invs and (\<lambda>s. rv \<longrightarrow> ct_running s) and
            (\<lambda>s. \<forall>x\<in>ran (kheap s). obj_valid_pdpt x)" in bind_wp_fwd)
        apply (wpsimp wp: check_budget_restart_true)
@@ -1738,7 +1742,9 @@ lemma call_kernel_valid_pdpt[wp]:
            (\<lambda>s. \<forall>x\<in>ran (kheap s). obj_valid_pdpt x) and
            (\<lambda>s. bound_sc_tcb_at (\<lambda>a. \<exists>y. a = Some y) (cur_thread s) s)" in bind_wp_fwd)
      apply wpsimp
-     apply (clarsimp simp: pred_tcb_at_def obj_at_def schedulable_def')
+     apply (clarsimp simp: pred_tcb_at_def obj_at_def schedulable_def opt_pred_def opt_map_def
+                           tcbs_of_kh_def
+                    split: option.splits)
     apply (rule_tac Q'="\<lambda>rv. invs and (\<lambda>s. rv \<longrightarrow> ct_running s) and
            (\<lambda>s. \<forall>x\<in>ran (kheap s). obj_valid_pdpt x)" in bind_wp_fwd)
      apply (wpsimp wp: check_budget_restart_true)
